x64 ainvs: prove uniqueness of IOPortControlCaps
This invariant is currently proved on the Haskell level only. This
commit is in preparation of removing the invariant from the Haskell
level, crossing it over via assertions.

Signed-off-by: Gerwin Klein <gerwin.klein@proofcraft.systems>

proof/invariant-abstract/X64/ArchInvariants_AI.thy
@@ -1051,6 +1051,21 @@ definition
 where
   "valid_x64_irq_state irqState \<equiv> \<forall>irq > maxIRQ. irqState irq = IRQFree"
 
+
+(* Mainly used to discharge the Haskell assertion archMDBAssertions, which is
+   used in CRefine. The invariant says that there is only one IOPortControlCap
+   in the system. *)
+definition ioport_control_unique_2 :: "(cslot_ptr \<Rightarrow> cap option) \<Rightarrow> bool" where
+  "ioport_control_unique_2 caps \<equiv>
+     \<forall>p p'. caps p = Some (ArchObjectCap IOPortControlCap) \<longrightarrow>
+            caps p' = Some (ArchObjectCap IOPortControlCap) \<longrightarrow>
+            p' = p"
+
+locale_abbrev ioport_control_unique where
+  "ioport_control_unique s \<equiv> ioport_control_unique_2 (caps_of_state s)"
+
+lemmas ioport_control_unique_def = ioport_control_unique_2_def
+
 definition
   valid_arch_state :: "'z::state_ext state \<Rightarrow> bool"
 where
@@ -1062,6 +1077,7 @@ where
       \<and> valid_global_pdpts s
       \<and> valid_cr3 (x64_current_cr3 (arch_state s))
       \<and> valid_x64_irq_state (x64_irq_state (arch_state s))
+      \<and> ioport_control_unique s
       \<and> valid_ioports s"
 
 definition
@@ -1778,23 +1794,23 @@ lemma valid_arch_state_lift:
    apply (wp arch typs caps hoare_vcg_conj_lift hoare_vcg_const_Ball_lift)+
   done
 
-(* we usually have a rule for valid_ioports, but it often comes with side-conditions *)
+(* we usually have a rule for valid_ioports and ioport_control_unique, but they often come with
+   side-conditions *)
 lemma valid_arch_state_lift_ioports_typ_at:
-  fixes Q
   assumes typs: "\<And>T p. \<lbrace>typ_at (AArch T) p\<rbrace> f \<lbrace>\<lambda>_. typ_at (AArch T) p\<rbrace>"
   assumes arch: "\<And>P. \<lbrace>\<lambda>s. P (arch_state s)\<rbrace> f \<lbrace>\<lambda>_ s. P (arch_state s)\<rbrace>"
   assumes ports: "\<lbrace> Q \<rbrace> f \<lbrace>\<lambda>_. valid_ioports \<rbrace>"
-  shows "\<lbrace>valid_arch_state and Q\<rbrace> f \<lbrace>\<lambda>_. valid_arch_state\<rbrace>"
-  apply (simp add: valid_arch_state_def pred_conj_def)
+  assumes control: "\<lbrace> P \<rbrace> f \<lbrace>\<lambda>_. ioport_control_unique\<rbrace>"
+  shows "\<lbrace>valid_arch_state and Q and P\<rbrace> f \<lbrace>\<lambda>_. valid_arch_state\<rbrace>"
   apply (simp add: valid_arch_state_def valid_asid_table_def
                    valid_global_pts_def valid_global_pds_def valid_global_pdpts_def)
-  (* we need to do this piece-wise so we can grab
-     `valid_ioports_2 (caps_of_state x) (arch_state x) \<and> Q x` at the end *)
-  apply (rule hoare_vcg_conj_lift[rotated])+
-  apply (solves \<open>wpsimp wp: ports\<close>)
-  (* the rest are trivial once arch_state is lifted out *)
-  apply (rule hoare_lift_Pf2[where f="\<lambda>s. arch_state s", OF _ arch],
-         solves \<open>wp typs hoare_vcg_conj_lift hoare_vcg_const_Ball_lift\<close>)+
+  apply wp_pre
+   (* isolate the `valid_ioports_2 (caps_of_state s) (arch_state s)` at the end,
+      because we don't want wps to act on (arch_state s) there. *)
+   apply (rule hoare_vcg_conj_lift[rotated])+
+            apply (rule ports)
+           apply (wps arch | wp control typs hoare_vcg_op_lift)+
+  apply simp
   done
 
 lemma aobj_at_default_arch_cap_valid:
